src/code/sys_verif_code/iterator.v
@@ -59,9 +59,29 @@ Definition mainⁱᵐᵖˡ : val :=
   λ: <>,
     exception_do (do:  #()).
 
-Definition isAscii : go_string := "sys_verif_code/iterator.isAscii"%go.
+Definition sliceIter : go_string := "sys_verif_code/iterator.sliceIter"%go.
 
 (* go: traceIter.go:3:6 *)
+Definition sliceIterⁱᵐᵖˡ : val :=
+  λ: "V" "s",
+    exception_do (let: "s" := (mem.alloc "s") in
+    return: ((λ: "yield",
+       exception_do (let: "yield" := (mem.alloc "yield") in
+       let: "$range" := (![#sliceT] "s") in
+       (let: "v" := (mem.alloc (type.zero_val "V")) in
+       slice.for_range "V" "$range" (λ: "$key" "$value",
+         do:  ("v" <-["V"] "$value");;;
+         do:  "$key";;;
+         (if: (~ (let: "$a0" := (!["V"] "v") in
+         (![#funcT] "yield") "$a0"))
+         then return: (#())
+         else do:  #())));;;
+       return: #())
+       ))).
+
+Definition isAscii : go_string := "sys_verif_code/iterator.isAscii"%go.
+
+(* go: traceIter.go:13:6 *)
 Definition isAsciiⁱᵐᵖˡ : val :=
   λ: "str",
     exception_do (let: "str" := (mem.alloc "str") in
@@ -69,9 +89,9 @@ Definition isAsciiⁱᵐᵖˡ : val :=
     let: "$r0" := #true in
     do:  ("ret_val" <-[#boolT] "$r0");;;
     let: "loop_body" := (mem.alloc (type.zero_val #funcT)) in
-    let: "$r0" := (λ: "i",
-      exception_do (let: "i" := (mem.alloc "i") in
-      (if: ((![#byteT] (slice.elem_ref #byteT (![#sliceT] "str") (![#intT] "i"))) ≥ #(W8 128)) || ((![#byteT] (slice.elem_ref #byteT (![#sliceT] "str") (![#intT] "i"))) = #(W8 0))
+    let: "$r0" := (λ: "b",
+      exception_do (let: "b" := (mem.alloc "b") in
+      (if: ((![#byteT] "b") ≥ #(W8 128)) || ((![#byteT] "b") = #(W8 0))
       then
         let: "$r0" := #false in
         do:  ("ret_val" <-[#boolT] "$r0");;;
@@ -83,9 +103,8 @@ Definition isAsciiⁱᵐᵖˡ : val :=
       ) in
     do:  ("loop_body" <-[#funcT] "$r0");;;
     let: "iterator" := (mem.alloc (type.zero_val #funcT)) in
-    let: "$r0" := (let: "$a0" := (let: "$a0" := (![#sliceT] "str") in
-    slice.len "$a0") in
-    (func_call #intIter) "$a0") in
+    let: "$r0" := (let: "$a0" := (![#sliceT] "str") in
+    ((func_call #sliceIter) #byteT) "$a0") in
     do:  ("iterator" <-[#funcT] "$r0");;;
     do:  (let: "$a0" := (![#funcT] "loop_body") in
     (![#funcT] "iterator") "$a0");;;
@@ -93,7 +112,7 @@ Definition isAsciiⁱᵐᵖˡ : val :=
 
 Definition vars' : list (go_string * go_type) := [].
 
-Definition functions' : list (go_string * val) := [(intIter, intIterⁱᵐᵖˡ); (factorial, factorialⁱᵐᵖˡ); (main, mainⁱᵐᵖˡ); (isAscii, isAsciiⁱᵐᵖˡ)].
+Definition functions' : list (go_string * val) := [(intIter, intIterⁱᵐᵖˡ); (factorial, factorialⁱᵐᵖˡ); (main, mainⁱᵐᵖˡ); (sliceIter, sliceIterⁱᵐᵖˡ); (isAscii, isAsciiⁱᵐᵖˡ)].
 
 Definition msets' : list (go_string * (list (go_string * val))) := [].
 
