src/generatedproof/sys_verif_code/iterator.v
@@ -42,6 +42,10 @@ Global Instance wp_func_call_main :
   WpFuncCall iterator.main _ (is_pkg_defined iterator) :=
   ltac:(solve_wp_func_call).
 
+Global Instance wp_func_call_sliceIter :
+  WpFuncCall iterator.sliceIter _ (is_pkg_defined iterator) :=
+  ltac:(solve_wp_func_call).
+
 Global Instance wp_func_call_isAscii :
   WpFuncCall iterator.isAscii _ (is_pkg_defined iterator) :=
   ltac:(solve_wp_func_call).
