src/iter/detTraceIter.v
@@ -1,0 +1,157 @@
+From sys_verif.program_proof Require Import prelude empty_ffi.
+From New.proof Require Import std.
+From New.generatedproof.sys_verif_code Require Import iterator.
+
+Section proof.
+Context `{hG: !heapGS Σ} `{!globalsGS Σ} {go_ctx: GoContext}.
+
+#[global] Instance : IsPkgInit iterator := define_is_pkg_init True%I.
+#[global] Instance : GetIsPkgInitWf iterator := build_get_is_pkg_init_wf.
+
+Definition is_detTraceIter V `{!IntoVal V} (detTraceIter yield : func.t) (trace : list V) (P : list V → iPropI Σ) Φ : iPropI Σ :=
+  (
+    "HP" :: P([]) ∗
+    "#Hyield" :: □(
+      ∀ (v : V) (vs : list V),
+        (⌜ vs ≠ trace ⌝ ∗ P(vs)) -∗
+        WP #yield #v {{ 
+          ok,
+          if (decide (ok = #true)) then
+            P((vs ++ [v])%list)
+          else if (decide (ok = #false)) then
+            Φ
+          else
+            False
+        }}
+    ) ∗
+    "Hlimit" :: (P(trace) -∗ Φ) 
+  )%I -∗
+  WP #detTraceIter #yield {{
+    _, Φ
+  }}.
+
+(* TODO: suprised that this isn't in the Rocq stdlib but the converse is? maybe should upstream? *)
+Lemma firstn_n_length :
+  ∀ (A : Type) (i : nat) (l : list A), take i l = l -> i >= length l.
+Proof.
+  induction i.
+  - intros l Htake.
+    rewrite firstn_0 in Htake.
+    subst.
+    simpl.
+    lia.
+  - induction l.
+    + simpl.
+      intros ?.
+      lia.
+    + rewrite firstn_cons.
+      intros ?.
+      assert (take i l = l) by congruence.
+      simpl.
+      apply IHi in H0.
+      lia.
+Qed.
+
+Lemma wp_sliceIter yield slice vs P Φ' :
+  {{{ 
+    is_pkg_init iterator ∗ 
+    "#Hslice" :: own_slice slice DfracDiscarded vs
+  }}}
+    @! iterator.sliceIter #uint8T #slice
+  {{{
+    (f : func.t), RET #f;
+    is_detTraceIter w8 f yield vs P Φ'
+  }}}.
+Proof.
+  wp_start.
+  iNamed "Hpre".
+  wp_auto.
+  iApply "HΦ".
+  unfold is_detTraceIter.
+  iIntros "Hpre".
+  iNamed "Hpre".
+  iDestruct (own_slice_len slice DfracDiscarded vs with "Hslice") as "[%Hlength %Hslice_len]".
+  wp_auto.
+  iAssert (
+    ∃(i : w64) (v : w8),
+    "i" :: i_ptr ↦ i ∗
+    "v" :: v_ptr ↦ v ∗
+    "HP" :: P(firstn (sint.nat i) vs) ∗
+    "%Hi" :: ⌜ 0 ≤ sint.Z i ≤ length vs ⌝
+  )%I with "[HP i v]" as "Hinv".
+  {
+    iFrame.
+    replace (sint.Z (W64 0)) with 0 by word.
+    word.
+  }
+  wp_for "Hinv".
+  wp_if_destruct.
+  {
+    wp_bind (slice.elem_ref (# uint8T) (# slice) (# i)).
+    wp_pure ; first word.
+    wp_auto.
+
+    (* TODO: cleanup *)
+    assert (sint.nat i < length vs)%nat as Hi2 by word.
+    pose proof (lookup_lt_is_Some_2 vs (sint.nat i)).
+    apply H in Hi2.
+    unfold is_Some in Hi2.
+    destruct Hi2.
+
+    wp_apply (wp_load_slice_elem slice i vs DfracDiscarded x) ; first lia.
+    {
+      iSplitL.
+      - iApply "Hslice".
+      - done.
+    }
+    iIntros "_".
+    wp_auto.
+    wp_bind (#yield (#_)).
+    iApply (wp_wand with "[HP]").
+    {
+      iApply "Hyield".
+      iFrame.
+      iPureIntro.
+      intuition.
+      assert (sint.nat i >= length vs).
+      {
+        apply firstn_n_length.
+        done.
+      }
+      lia.
+    }
+    iIntros (?) "Hpost".
+    destruct (decide _).
+    {
+      subst.
+      wp_auto.
+      wp_for_post.
+      iFrame.
+      iSplitL.
+      - replace (sint.nat (word.add i (W64 1))) with (S (sint.nat i))%nat by word.
+        simpl.
+        Search "take".
+        assert (take (S (sint.nat i)) vs = take (sint.nat i) vs ++ [x]).
+        {
+          apply take_S_r.
+          done.
+        }
+        rewrite H1.
+        done.
+      - word.
+    }
+    destruct (decide _).
+    {
+      subst.
+      wp_auto.
+      wp_for_post.
+      iFrame.
+    }
+    done.
+  }
+  iApply "Hlimit".
+  replace (sint.nat i) with (length vs) by word.
+  - assert (take (length vs) vs = vs) by apply firstn_all.
+    replace (take (length vs) vs) with vs.
+    done.
+Qed.
